progs/verif1.v
@@ -26,31 +26,43 @@ Defined.
 
 Definition int2valt (i: int) := (Vint i, P.t_int).
 
+Definition ilseg (s: list int) p q := lseg P.t_listptr (map Vint s) p q.
+
+(*
+Definition ilseg (s: list int) (p q: expr) : assert
+   := fun rho => lseg P.t_listptr (map Vint s) (eval_expr rho p) (eval_expr rho q).
+*)
+
 Definition sumlist_spec :=
  DECLARE P.i_sumlist
   WITH contents 
-  PRE [ p : P.t_listptr]  lseg (map (fun i => (Vint i, P.t_int)) contents) (p, P.t_listptr) (nullval, P.t_listptr)
+  PRE [ p : P.t_listptr]  ilseg contents p nullval
   POST [ i : P.t_int ] prop (i = Vint (fold_right Int.add Int.zero contents)).
 
 Definition reverse_spec :=
  DECLARE P.i_reverse
   WITH contents : list int
-  PRE  [ p : P.t_listptr ] lseg (map int2valt contents) (p, P.t_listptr) (nullval, P.t_listptr)
-  POST [p : P.t_listptr ] lseg (map int2valt (rev contents)) (p, P.t_listptr) (nullval, P.t_listptr).
+  PRE  [ p : P.t_listptr ] ilseg contents p nullval
+  POST [p : P.t_listptr ] ilseg (rev contents) p nullval.
 
 Definition main_spec := (P.i_main, mk_funspec (Tnil, P.t_int) _ (main_pre P.prog) (main_post P.prog)).
 
 Definition Gprog : funspecs := 
    sumlist_spec :: reverse_spec :: main_spec::nil.
 
-Definition sumlist_Inv (contents: list int) (rho: environ) : mpred :=
+Definition sumlist_Inv (contents: list int) : assert :=
+          (EX cts: list int, 
+           (fun rho => !!(fold_right Int.add Int.zero contents =
+             Int.add (force_int (eval_expr rho (Etempvar P.i_s P.t_int)))
+                       (fold_right Int.add Int.zero cts))) &&
+           (fun rho => ilseg cts (eval_expr rho (Etempvar P.i_t P.t_listptr)) nullval)).
+
+Definition sumlist_Inv' (contents: list int) (rho: environ) : mpred :=
           (EX cts: list int, 
            !!(fold_right Int.add Int.zero contents =
              Int.add (force_int (eval_expr rho (Etempvar P.i_s P.t_int)))
                        (fold_right Int.add Int.zero cts)) &&
-           lseg (map (fun i => (Vint i, P.t_int)) cts) 
-                 (eval_expr rho (Etempvar P.i_t P.t_listptr), P.t_listptr)
-                 (nullval, P.t_listptr)).
+           ilseg cts (eval_expr rho (Etempvar P.i_t P.t_listptr)) nullval).
 
 Definition semax_body' (G:  funspecs) (f: function) (spec: ident * funspec) :=
   match spec with (i, mk_funspec _ A pre post) => semax_body G f A pre post end.
@@ -64,100 +76,208 @@ Lemma typecheck_val_ptr_lemma:
 Proof.
 Admitted.
 
+(*
+Lemma bool_val_notbool_ptr:
+    forall v t a,
+   (bool_val (force_val (sem_notbool v (Tpointer t a))) type_bool = Some true) = (v = nullval).
+Proof.
+ intros.
+ apply prop_ext; split; intros.
+ destruct v; simpl in H; try discriminate.
+ apply bool_val_int_eq_e in H. subst; auto.
+ subst. simpl. auto.
+Qed.
+*)
+
+Lemma bool_val_notbool_ptr:
+    forall v t,
+   match t with Tpointer _ _ => True | _ => False end ->
+   (bool_val (force_val (sem_notbool v t)) type_bool = Some true) = (v = nullval).
+Proof.
+ intros.
+ destruct t; try contradiction. clear H.
+ apply prop_ext; split; intros.
+ destruct v; simpl in H; try discriminate.
+ apply bool_val_int_eq_e in H. subst; auto.
+ subst. simpl. auto.
+Qed.
+
+Hint Rewrite bool_val_notbool_ptr using (solve [simpl; auto]) : normalize.
+Hint Rewrite Int.add_zero  Int.add_zero_l Int.sub_zero_l : normalize.
+
+Lemma lseg_unroll': forall T {ls: listspec T} l x z , 
+    lseg T l x z = (!! (ptr_eq x z) && !! (l=nil) && emp) || 
+                          (EX h:val, EX r:list val, EX y:val, 
+                          !! (~ptr_eq x z) &&  !!(l=h::r) && 
+                       field_mapsto Share.top (x, list_struct) list_data (h, list_dtype) 
+                      * field_mapsto Share.top (x, list_struct) list_link (y, T)
+                      * |> lseg T r y z).
+Proof.
+intros.
+rewrite lseg_unfold at 1.
+apply pred_ext; destruct l.
+normalize.
+apply orp_right1; auto.
+apply orp_right2.
+apply exp_right with v.
+apply exp_right with l.
+normalize. intro y.
+apply exp_right with y.
+normalize.
+apply orp_left; auto.
+normalize.
+normalize.
+intros. inv H0.
+apply orp_left.
+normalize.
+inv H0.
+normalize.
+intros.
+inv H0.
+apply exp_right with x2.
+normalize.
+Qed.
+
+Definition ilseg_nil (l: list  int) x z := !! (ptr_eq x z) && !! (l=nil) && emp.
+Definition ilseg_cons l x z := 
+                          (EX h:int, EX r:list int, EX y:val, 
+                          !! (~ptr_eq x z) &&  !!(l=h::r) && 
+                       field_mapsto Share.top (x, list_struct) list_data (Vint h, P.t_int) 
+                      * field_mapsto Share.top (x, list_struct) list_link (y, P.t_listptr)
+                      * |> ilseg r y z).
+
+Lemma ilseg_unroll': forall l x z , 
+    ilseg l x z = ilseg_nil l x z || ilseg_cons l x z.
+Proof.
+intros.
+unfold ilseg at 1.
+rewrite lseg_unroll'.
+unfold ilseg_cons, ilseg_nil, ilseg.
+f_equal.
+f_equal. f_equal.
+f_equal.
+apply prop_ext; split; intro; destruct l; simpl in *; congruence.
+apply pred_ext; normalize.
+intros h r ? y. destruct l; inv H0.
+apply exp_right with i.
+apply exp_right with l.
+apply exp_right with y.
+normalize.
+intros h r y.
+apply exp_right with (Vint h).
+apply exp_right with (map Vint r).
+apply exp_right with y.
+simpl.
+normalize.
+Qed.
+
+
+Lemma semax_pre':
+ forall (P': assert) Delta G (P: assert) c R,
+   (fun rho => !! (typecheck_environ rho Delta = true)) && P |-- P' ->   
+  semax Delta G P' c R  -> semax Delta G P c R.
+Proof. intros; apply semax_pre with P'; auto. 
+intros.
+eapply derives_trans; [ | apply H].
+simpl; apply andp_right; auto.
+normalize.
+Qed.
+
+Lemma expr_true_Cnot_ptr: 
+  forall e, match typeof e with Tpointer _ _ => True | _ => False end ->
+     forall rho,  (expr_true (Cnot e) rho) = (eval_expr rho e = nullval).
+Proof.
+intros.
+ unfold expr_true, Cnot.
+ apply bool_val_notbool_ptr; auto.
+Qed.
+Hint Rewrite expr_true_Cnot_ptr using (solve [simpl; auto]) : normalize.
+
+Lemma expr_true_Cnot_ptr': 
+  forall e, match typeof e with Tpointer _ _ => True | _ => False end ->
+    local (expr_true (Cnot e)) = local (fun rho => eval_expr rho e = nullval).
+Proof.
+ intros. extensionality rho. unfold local. f_equal. apply expr_true_Cnot_ptr; auto.
+Qed.
+Hint Rewrite expr_true_Cnot_ptr' using (solve [simpl; auto]) : normalize.
+
+Lemma local_unfold: forall P rho, local P rho = !! (P rho).
+Proof. reflexivity. Qed.
+Hint Rewrite local_unfold : normalize.
+
 Lemma body_sumlist: semax_body' Gprog P.f_sumlist sumlist_spec.
 Proof.
 intro contents.
 simpl fn_body; simpl fn_params; simpl fn_return.
 normalize.
-apply forward_set; [compute; auto | compute; auto | auto with closed | normalize | ].
-apply forward_set; [compute; auto | compute; auto | auto with closed | normalize | ].
+apply forward_set; [compute; auto | compute; auto | auto with closed | compute; auto | ].
+apply forward_set; [compute; auto | compute; auto | auto with closed | compute; auto | ].
 forward_while (sumlist_Inv contents)
     (fun rho => !!(fold_right Int.add Int.zero contents = force_int (eval_id rho P.i_s))).
-
+(* Prove that current precondition implies loop invariant *)
 unfold sumlist_Inv; intros; simpl; normalize.
 apply exp_right with contents.
 rewrite H0. rewrite H1.  simpl.
 rewrite Int.add_zero_l. normalize.
-
+(* Prove that loop invariant implies typechecking condition *)
 intros; unfold tc_expr; simpl; normalize.
+(* Prove that invariant && not loop-cond implies postcondition *)
 intro rho.
 normalize.
-unfold Cnot, expr_true.
-normalize.
-simpl in H.
-assert (eval_id rho P.i_t = nullval).
-destruct (eval_id rho P.i_t); simpl in H; try discriminate.
-apply bool_val_int_eq_e in H. subst; auto.
 unfold sumlist_Inv.
+simpl.
 apply exp_left; intro cts.
 normalize.
 rewrite H0.
-rewrite (lseg_eq (map (fun i : int => (Vint i, P.t_int)) cts) nullval P.t_listptr).
-rewrite H1.
+rewrite H.
+unfold ilseg; rewrite lseg_eq; auto.
 normalize.
-destruct cts; inv H2.  simpl fold_right. 
-rewrite Int.add_zero.  normalize.
-simpl. apply Int.eq_true.
-eapply sequential; [intros; simpl; reflexivity | ].
-unfold sumlist_Inv at 1.
-apply semax_pre with 
-   (fun rho : environ =>
-    (EX  cts : list int,
-    expr_true (Etempvar P.i_t P.t_listptr) rho &&
-    !!(fold_right Int.add Int.zero contents =
-       Int.add (force_int (eval_expr rho (Etempvar P.i_s P.t_int)))
-         (fold_right Int.add Int.zero cts)) &&
-    lseg (map (fun i : int => (Vint i, P.t_int)) cts)
-      (eval_id rho P.i_t, P.t_listptr)
-      (nullval, P.t_listptr))).
-intro; normalize; intros.
-apply exp_right with x.
-normalize.
-apply extract_exists_pre.
-apply nil.
-intro cts.
+destruct cts; inv H1. simpl. normalize.
+(* Prove that loop body preserves invariant *)
+unfold sumlist_Inv at 1. normalize.
+apply extract_exists_pre; auto;  intro cts.
 
-pose (P' rho := 
-(EX  h : val,
- (EX  r : list valt,
-  (EX  y : val,
-    expr_true (Etempvar P.i_t P.t_listptr) rho &&
-!!(fold_right Int.add Int.zero contents =
-   Int.add (force_int (eval_expr rho (Etempvar P.i_s P.t_int)))
-     (fold_right Int.add Int.zero cts)) &&
-   !!(map (fun i : int => (Vint i, P.t_int)) cts = (h, P.t_int) :: r /\
-      typecheck_val h P.t_int = true /\ typecheck_val y P.t_listptr = true) &&
-   field_mapsto Share.top
-     (eval_expr rho (Etempvar P.i_t P.t_listptr), P.t_list) P.i_h
-     (h, P.t_int) *
-   field_mapsto Share.top
-     (eval_expr rho (Etempvar P.i_t P.t_listptr), P.t_list) P.i_t
-     (y, P.t_listptr) * |>lseg r (y, P.t_listptr) (nullval, P.t_listptr))))).
-apply semax_pre with P'; unfold P' in *; clear P'.
-intros.
-unfold expr_true.
-normalize.
-rewrite lseg_neq.
-normalize.
-intros h r y.
-normalize. apply (exp_right h).
-normalize. apply (exp_right r).
-normalize. apply (exp_right y).
-normalize.
-clear - H H0.
-simpl in *.
-eapply typecheck_val_ptr_lemma; eauto; simpl; reflexivity.
-simpl. apply Int.eq_true.
+apply semax_pre with
+(local (expr_true (Etempvar P.i_t P.t_listptr)) &&
+ (fun rho => !!(fold_right Int.add Int.zero contents =
+       Int.add (force_int (eval_id rho P.i_s))
+         (fold_right Int.add Int.zero cts))) &&
+ (fun rho => ilseg_cons cts (eval_id rho P.i_t) nullval)).
 intro.
-unfold ptr_eq in H2.
-destruct (eval_id rho P.i_t); try contradiction.
-simpl in H2.
-simpl in H0.
-rewrite H2 in H0. inv H0.
+simpl.
+rewrite ilseg_unroll'. auto.
+unfold ilseg_cons, ilseg_nil.
+intro.
+normalize.
+apply orp_left.
+normalize.
+unfold expr_true, bool_val in H1. simpl in H1.
+unfold ptr_eq in H2. destruct (eval_id rho P.i_t); simpl in *; try contradiction.
+rewrite H2 in H1; inv H1.
+normalize. intros h r ? y.
+apply exp_right with h; normalize. apply exp_right with r; normalize.
+apply exp_right with y; normalize.
+unfold ilseg_cons.
+match goal with |- semax _ _ (_ && _ && ?P) _ _ => 
+  change P with (EX  h : int, EX  r : list int, EX  y : val,  
+      fun rho => !!(~ ptr_eq (eval_id rho P.i_t) nullval) && !!(cts = h :: r) &&
+      field_mapsto Share.top (eval_id rho P.i_t, list_struct) list_data
+        (Vint h, P.t_int) *
+      field_mapsto Share.top (eval_id rho P.i_t, list_struct) list_link
+        (y, P.t_listptr) * |>ilseg r y nullval)
+ end.
+normalize. apply extract_exists_pre; [apply Int.zero | intro h].
+normalize. apply extract_exists_pre; [apply nil | intro r].
+normalize. apply extract_exists_pre; [apply Vundef | intro y].
+simpl.
 
-apply extract_exists_pre; [apply Vundef |  intro h].
-apply extract_exists_pre; [apply nil |  intro r].
-apply extract_exists_pre; [apply Vundef |  intro y].
+match goal with |- semax _ _ ?P _ _ => 
+  apply semax_pre with (!!(cts = h::r) && P)
+end.
+intro; normalize.
+apply semax_extract_prop.
+intro; subst cts.
+
 apply semax_pre with
   (fun rho : environ =>
   !!(map (fun i : int => (Vint i, P.t_int)) cts = (h, P.t_int) :: r /\
@@ -166,12 +286,9 @@ apply semax_pre with
    !!(fold_right Int.add Int.zero contents =
       Int.add (force_int (eval_id rho P.i_s))
         (fold_right Int.add Int.zero cts)) &&
-   field_mapsto Share.top
-     (eval_id rho P.i_t, P.t_list) P.i_h
-     (h, P.t_int) *
-   field_mapsto Share.top
-     (eval_id rho P.i_t, P.t_list) P.i_t
-     (y, P.t_listptr) * |>lseg r (y, P.t_listptr) (nullval, P.t_listptr))).
+   field_mapsto Share.top (eval_id rho P.i_t, P.t_list) P.i_h  (h, P.t_int) *
+   field_mapsto Share.top (eval_id rho P.i_t, P.t_list) P.i_t  (y, P.t_listptr) *
+     |>lseg r (y, P.t_listptr) (nullval, P.t_listptr))).
 intros.
 unfold expr_true.
 normalize.
@@ -198,6 +315,7 @@ apply semax_pre with
 intros.
 
 admit.
+eapply sequential; [intros; simpl; reflexivity | ].
 pose (Q := 
        ((fun rho => field_mapsto Share.top ((eval_lvalue rho e1), typeof e1) P.i_h (h, P.t_int)) * P)).
 apply semax_seq with Q.
